fun_defs.v
@@ -46,7 +46,7 @@ Notation ø := fe_null.
 Notation " x '#' y " := (fe_pair x y) (at level 26, y at level 0, format "x # y", right associativity) : expr_scope.
 Notation " 'MATCH' e 'WITH' 'ø' ⇒ a 'OR' x '#' y ⇒ b " := (fe_match e a x y b) (at level 29, format "MATCH  e  WITH  ø  ⇒  a  OR  x # y  ⇒  b", x at level 0, y at level 0) : expr_scope. 
 
-Notation " 'LET' x '::=' y 'IN' z " := (fe_let x y z) (at level 25, format "LET  x ::= y  IN z", x at level 0, y at level 0, z at level 0) : expr_scope.
+Notation " 'LET' x '::=' y 'IN' z " := (fe_let x y z) (at level 25, format "LET  x ::= y  IN  z", x at level 0, y at level 0, z at level 0) : expr_scope.
 Notation " 'CALL' f 'ON' x " := (fe_call  f x) (at level 25, f at level 0, format "CALL  f  ON  x", x at level 0) : expr_scope.
 
 Open Scope expr_scope.
@@ -81,6 +81,30 @@ Section fun_sem.
   Fact fs_var x e a : e⇢x = a -> £x // e ~~> a.
   Proof. intros []; constructor. Qed.
 
+  Fact fun_sem_var_inv x e a : £x // e ~~> a -> a = e⇢x.
+  Proof. inversion 1; auto. Qed.
+
+  Fact fun_sem_null_inv e a : ø // e ~~> a -> a = ω.
+  Proof. inversion 1; auto. Qed.
+
+  Fact fun_sem_pair_inv f g e v : f#g// e ~~> v -> exists a b, v = ⟨a,b⟩ /\ f // e ~~> a /\ g // e ~~> b.
+  Proof. inversion 1; exists a, b; auto. Qed.
+ 
+  Fact fun_sem_match_inv f u x y v e c :
+        MATCH f WITH ø⇒u OR x#y⇒v // e ~~> c -> f // e ~~> ω /\ u // e ~~> c 
+                                 \/ exists a b, f // e ~~> ⟨a,b⟩ /\ v // e⦃x⇠a⦄⦃y⇠b⦄ ~~> c.
+  Proof.
+    inversion 1.
+    + left; auto.
+    + right; exists a, b; auto.
+  Qed.
+
+  Fact fun_sem_let_inv x f g e v : LET x::=f IN g // e ~~> v -> exists a, f // e ~~> a /\ g // e⦃x⇠a⦄ ~~> v.
+  Proof. inversion 1; exists a; auto. Qed.
+  
+  Fact fun_sem_call_inv fi g e v : CALL fi ON g // e ~~> v -> exists a, g // e ~~> a /\ body fi // e⦃param fi⇠a⦄ ~~> v.
+  Proof. inversion 1; exists a; auto. Qed.
+
   Fact fun_sem_det f e a b : f // e ~~> a -> f // e ~~> b -> a = b.
   Proof.
     intros H1; revert H1 b.
@@ -91,20 +115,54 @@ Section fun_sem.
                    | f u x y v e a b c H1 IH1 H2 IH2 
                    | x f g e a b H1 IH1 H2 IH2 
                    | p g e a b H1 IH1 H2 IH2 ].
-    + inversion 1; auto.
-    + inversion 1; auto.
-    + inversion 1; f_equal; auto.
-    + inversion 1; auto.
-      apply IH1 in H9; discriminate.
-    + inversion 1.
-      * apply IH1 in H9; discriminate.
-      * apply IH1 in H9; inversion H9; subst.
-        apply IH2 in H10; auto.
-    + inversion 1.
-      apply IH1 in H7; subst; auto.
-    + inversion 1.
-      apply IH1 in H4; subst.
-      apply IH2 in H7; subst; auto.
+    + intros v H; apply fun_sem_var_inv in H; auto.
+    + intros v H; apply fun_sem_null_inv in H; auto.
+    + intros v H; apply fun_sem_pair_inv in H.
+      destruct H as (a' & b' & H3 & H4 & H5); subst; f_equal; auto.
+    + intros c H.
+      apply fun_sem_match_inv in H.
+      destruct H as [ (H3 & H4) | (a' & b' & H3 & H4) ]; auto.
+      apply IH1 in H3; discriminate.
+    + intros w H.
+      apply fun_sem_match_inv in H.
+      destruct H as [ (H3 & H4) | (a' & b' & H3 & H4) ].
+      * apply IH1 in H3; discriminate.
+      * apply IH1 in H3; inversion H3.
+        apply IH2; subst; auto.
+    + intros v H.
+      apply fun_sem_let_inv in H.
+      destruct H as (a' & H3 & H4).
+      apply IH1 in H3; subst; auto.
+    + intros v H.
+      apply fun_sem_call_inv in H.
+      destruct H as (a' & H3 & H4).
+      apply IH1 in H3; subst; auto.
   Qed.
+
+  Section loop.
+
+    Variables (p : Var) (loop : Fun) (Hloop1 : param loop = p) (Hloop2 : body loop = CALL loop ON £p).
+
+    Let loop_does_not_stop f e a : f // e ~~> a -> forall e', f = CALL loop ON e' -> False.
+    Proof.
+      induction 1 as [ x e 
+                     | e 
+                     | f g e a b H1 IH1 H2 IH2 
+                     | f u x y v e a H1 IH1 H2 IH2 
+                     | f u x y v e a b c H1 IH1 H2 IH2 
+                     | x f g e a b H1 IH1 H2 IH2 
+                     | fi g e a b H1 IH1 H2 IH2 ]; intros e'; try discriminate.
+      inversion 1; subst fi g.
+      rewrite Hloop2 in IH2.
+      apply (IH2 _ eq_refl).
+    Qed.
+ 
+    Theorem loop_spec f e a : ~ CALL loop ON f // e ~~> a.
+    Proof.
+      intros H.
+      apply loop_does_not_stop with (1 := H) (2 := eq_refl).
+    Qed.
+
+  End loop.
 
 End fun_sem.
